Port to micro, fix proofs

CpcMicro/SmtModel.lean
@@ -236,8 +236,8 @@ inductive SmtTerm : Type where
   | Binary : native_Int -> native_Int -> SmtTerm
   | Apply : SmtTerm -> SmtTerm -> SmtTerm
   | Var : native_String -> SmtType -> SmtTerm
-  | ite : SmtTerm
-  | eq : SmtTerm
+  | ite : SmtTerm -> SmtTerm -> SmtTerm -> SmtTerm
+  | eq : SmtTerm -> SmtTerm -> SmtTerm
   | exists : native_String -> SmtType -> SmtTerm
   | forall : native_String -> SmtType -> SmtTerm
   | choice : native_String -> SmtType -> SmtTerm
@@ -501,8 +501,8 @@ def __smtx_typeof : SmtTerm -> SmtType
   | (SmtTerm.or x1 x2) => (native_ite (native_Teq (__smtx_typeof x1) SmtType.Bool) (native_ite (native_Teq (__smtx_typeof x2) SmtType.Bool) SmtType.Bool SmtType.None) SmtType.None)
   | (SmtTerm.and x1 x2) => (native_ite (native_Teq (__smtx_typeof x1) SmtType.Bool) (native_ite (native_Teq (__smtx_typeof x2) SmtType.Bool) SmtType.Bool SmtType.None) SmtType.None)
   | (SmtTerm.imp x1 x2) => (native_ite (native_Teq (__smtx_typeof x1) SmtType.Bool) (native_ite (native_Teq (__smtx_typeof x2) SmtType.Bool) SmtType.Bool SmtType.None) SmtType.None)
-  | (SmtTerm.Apply (SmtTerm.Apply (SmtTerm.Apply SmtTerm.ite x1) x2) x3) => (__smtx_typeof_ite (__smtx_typeof x1) (__smtx_typeof x2) (__smtx_typeof x3))
-  | (SmtTerm.Apply (SmtTerm.Apply SmtTerm.eq x1) x2) => (__smtx_typeof_eq (__smtx_typeof x1) (__smtx_typeof x2))
+  | (SmtTerm.ite x1 x2 x3) => (__smtx_typeof_ite (__smtx_typeof x1) (__smtx_typeof x2) (__smtx_typeof x3))
+  | (SmtTerm.eq x1 x2) => (__smtx_typeof_eq (__smtx_typeof x1) (__smtx_typeof x2))
   | (SmtTerm.Apply (SmtTerm.exists s T) x1) => (native_ite (native_Teq (__smtx_typeof x1) SmtType.Bool) SmtType.Bool SmtType.None)
   | (SmtTerm.Apply (SmtTerm.forall s T) x1) => (native_ite (native_Teq (__smtx_typeof x1) SmtType.Bool) SmtType.Bool SmtType.None)
   | (SmtTerm.Apply (SmtTerm.choice s T) x1) => (native_ite (native_Teq (__smtx_typeof x1) SmtType.Bool) (__smtx_typeof_guard_inhabited T T) SmtType.None)
@@ -656,8 +656,8 @@ noncomputable def __smtx_model_eval (M : SmtModel) : SmtTerm -> SmtValue
   | (SmtTerm.or x1 x2) => (__smtx_model_eval_or (__smtx_model_eval M x1) (__smtx_model_eval M x2))
   | (SmtTerm.and x1 x2) => (__smtx_model_eval_and (__smtx_model_eval M x1) (__smtx_model_eval M x2))
   | (SmtTerm.imp x1 x2) => (__smtx_model_eval_imp (__smtx_model_eval M x1) (__smtx_model_eval M x2))
-  | (SmtTerm.Apply (SmtTerm.Apply (SmtTerm.Apply SmtTerm.ite x1) x2) x3) => (__smtx_model_eval_ite (__smtx_model_eval M x1) (__smtx_model_eval M x2) (__smtx_model_eval M x3))
-  | (SmtTerm.Apply (SmtTerm.Apply SmtTerm.eq x1) x2) => (__smtx_model_eval_eq (__smtx_model_eval M x1) (__smtx_model_eval M x2))
+  | (SmtTerm.ite x1 x2 x3) => (__smtx_model_eval_ite (__smtx_model_eval M x1) (__smtx_model_eval M x2) (__smtx_model_eval M x3))
+  | (SmtTerm.eq x1 x2) => (__smtx_model_eval_eq (__smtx_model_eval M x1) (__smtx_model_eval M x2))
   | (SmtTerm.Apply (SmtTerm.exists s T) x1) => (native_eval_texists M s T x1)
   | (SmtTerm.Apply (SmtTerm.forall s T) x1) => (native_eval_tforall M s T x1)
   | (SmtTerm.Apply (SmtTerm.choice s T) x1) => (native_eval_tchoice M s T x1)
